yam (yet another milestone): partitions of empty is singleton

Bell.lean
@@ -1,7 +1,7 @@
 import mathlib
 import Mathlib.Data.Finset.Powerset
 import Mathlib.Data.Fintype.Basic
-import Mathlib.Data.Nat.Choose.Basic -- For Nat.choose
+import Mathlib.Data.Nat.Choose.Basic
 import Mathlib.Tactic.Basic
 import Mathlib.Logic.Equiv.Option
 
@@ -70,20 +70,23 @@ lemma partition.mk_if_valid_id_family
     split_ifs at mk_is_some with h₁ h₂ h₃; simp only [Option.some_inj] at mk_is_some
     rw [← mk_is_some]
 
+
+lemma partition.mk_if_valid_inj_some {X: Type u} [DecidableEq X] (S: Finset X) :
+  ∀ (a a' : Finset (Finset X)), ∀ b ∈ mk_if_valid S a, b ∈ mk_if_valid S a' → a = a' :=
+by
+  intros fam1 fam2 p p_in_fam1 p_in_fam2
+  rw [Option.mem_def] at p_in_fam1 p_in_fam2
+
+  have fam_eq_fam1 : p.family = fam1 :=
+    partition.mk_if_valid_id_family S fam1 p p_in_fam1
+  have fam_eq_fam2 : p.family = fam2 :=
+    partition.mk_if_valid_id_family S fam2 p p_in_fam2
+
+  rw [← fam_eq_fam1, fam_eq_fam2]
+
 -- not the shortest neatier proof but it's constructive and educational
 instance partition.Fintype {X : Type u} [DecidableEq X] (S: Finset X) : Fintype (partition X S) where
-  elems := (S.powerset.powerset).filterMap (partition.mk_if_valid S) (
-    by
-      intros fam1 fam2 p p_in_fam1 p_in_fam2
-      rw [Option.mem_def] at p_in_fam1 p_in_fam2
-
-      have fam_eq_fam1 : p.family = fam1 :=
-        partition.mk_if_valid_id_family S fam1 p p_in_fam1
-      have fam_eq_fam2 : p.family = fam2 :=
-        partition.mk_if_valid_id_family S fam2 p p_in_fam2
-
-      rw [← fam_eq_fam1, fam_eq_fam2]
-  )
+  elems := (S.powerset.powerset).filterMap (partition.mk_if_valid S) (partition.mk_if_valid_inj_some S)
   complete := by
     intro part
     simp_rw [Finset.mem_filterMap]
@@ -137,7 +140,7 @@ def the_empty_partition (X : Type u) [DecidableEq X] : partition X ∅ := {
   disjoint := fun c hc => (Finset.not_mem_empty c hc).elim
 }
 
-lemma empty_powerset {X} [DecidableEq X]: (∅: Finset X).powerset = {∅} := by
+lemma singleton_empty_powerset {X} [DecidableEq X]: ({∅}: (Finset (Finset X))).powerset = {∅, {∅}} := by
   ext fam
   constructor
   · intro h
@@ -145,56 +148,172 @@ lemma empty_powerset {X} [DecidableEq X]: (∅: Finset X).powerset = {∅} := by
   · intro h
     exact h
 
-lemma empty_singleton_powerset {X} [DecidableEq X]: ({∅}: (Finset (Finset X))).powerset = {∅, {∅}} := by
-  ext fam
-  constructor
-  · intro h
-    exact h
-  · intro h
-    exact h
-
-lemma empty_double_powerset {X} [DecidableEq X]: (∅: Finset X).powerset.powerset = {∅, {∅}} := by
-  rw [empty_powerset, empty_singleton_powerset]
-
-lemma card_empty_partition {X: Type u} [DecidableEq X] : Fintype.card (partition X ∅) = 1 :=
+lemma filterMap_filter_isSome_eq_filterMap
+  {α β : Type*} [DecidableEq α] [DecidableEq β]
+  (s : Finset α)
+  (f : α → Option β)
+  (hf_inj : ∀ (a a' : α), ∀ (b : β), (f a = some b) → (f a' = some b) → a = a')
+: ((s.filter (fun x => (f x).isSome)).filterMap f hf_inj) = s.filterMap f hf_inj :=
 by
-  unfold Fintype.card Finset.univ partition.Fintype
-  let ppe := (∅: Finset X).powerset.powerset
-  have h : Finset.filter (fun fam => (partition.mk_if_valid ∅ fam).isSome) (∅: Finset X).powerset.powerset = {∅} := by
-    rw [empty_double_powerset]
-    ext fam
-    simp only [Finset.mem_filter, Finset.mem_insert, Finset.mem_singleton, or_iff_left_iff_imp, iff_def]
+  have filterMap_subset_filter_isSome_filterMap:
+    (s.filterMap f hf_inj) ⊆ (s.filter (fun x => (f x).isSome)).filterMap f hf_inj :=
+  by
+    intro y y_in_filterMap
+    rw [Finset.mem_filterMap] at y_in_filterMap
+    rcases y_in_filterMap with ⟨x, x_in_s, fx_is_some_y⟩
+    rw [Finset.mem_filterMap]
+    use x
     constructor
-    · intro h_conj
-      rcases h_conj with ⟨h_fam_cases, h_is_some⟩
-      cases h_fam_cases with
-      | inl h_fam_is_empty_family => exact h_fam_is_empty_family
-      | inr h_fam_contains_empty_set =>
-        have h_eval_invalid : (partition.mk_if_valid (∅ : Finset X) ({∅} : Finset (Finset X))).isSome = false := by
-          unfold partition.mk_if_valid
-          simp only [ne_eq, not_true, false_implies, Option.isSome_none]
-          simp
-        rw [h_fam_contains_empty_set] at h_is_some
-        rw [h_eval_invalid] at h_is_some
-        apply absurd h_is_some
-        -- TODO: figure out which tactics were used here
-        simp
+    .
+      rw [Finset.mem_filter]
+      constructor
+      . exact x_in_s
+      . simp only [Option.isSome_some, fx_is_some_y]
+    . exact fx_is_some_y
+
+  have filter_isSome_filterMap_subset_filterMap:
+    (s.filter (fun x => (f x).isSome)).filterMap f hf_inj ⊆ s.filterMap f hf_inj :=
+  by
+    intro y y_in_filterMap
+    rw [Finset.mem_filterMap] at y_in_filterMap
+    rcases y_in_filterMap with ⟨x, x_in_s_filter_isSome, fx_is_some_y⟩
+    rw [Finset.mem_filterMap]
+    use x
+    constructor
+    .
+      rw [Finset.mem_filter] at x_in_s_filter_isSome
+      exact And.left x_in_s_filter_isSome
+    . exact fx_is_some_y
+
+  apply Finset.Subset.antisymm_iff.mpr
+  constructor
+  . exact filter_isSome_filterMap_subset_filterMap
+  . exact filterMap_subset_filter_isSome_filterMap
+
+lemma filterMap_card_eq_filter_isSome_card
+  {α β : Type*} [DecidableEq α] [DecidableEq β]
+  (s : Finset α)
+  (f : α → Option β)
+  (hf_inj : ∀ (a a' : α), ∀ (b : β), (f a = some b) → (f a' = some b) → a = a')
+ : (s.filterMap f hf_inj).card = (s.filter (fun x => (f x).isSome)).card :=
+by
+  rw [Finset.card_bij (fun x _ => Option.get (f x) _)]
+  -- prove the function maps to the target set
+  ·
+    intro x hx
+    rw [Finset.mem_filter] at hx
+    obtain ⟨x_in_s, fx_isSome⟩ := hx
+    rw [Finset.mem_filterMap]
+    use x, x_in_s
+    simp only [Option.some_get fx_isSome]
+  -- prove injectivity
+  ·
+    intro x₁ hx₁ x₂ hx₂ h_eq
+    rw [Finset.mem_filter] at hx₁ hx₂
+    obtain ⟨x₁_in_s, x₁_isSome⟩ := hx₁
+    obtain ⟨x₂_in_s, x₂_isSome⟩ := hx₂
+    have h₁ : f x₁ = some (Option.get (f x₁) x₁_isSome) := by simp only [Option.some_get x₁_isSome]
+    have h₂ : f x₂ = some (Option.get (f x₂) x₂_isSome) := by simp only [Option.some_get x₂_isSome]
+    simp [Option.get_inj] at h_eq
+    apply hf_inj x₁ x₂ (Option.get (f x₁) x₁_isSome)
+    · simp only [Option.some_get x₁_isSome]
+    · simp only [Option.some_get x₂_isSome, h_eq]
+  -- prove surjectivity
+  ·
+    intro y hy
+    rw [Finset.mem_filterMap] at hy
+    obtain ⟨x, hx_in_s, hfx⟩ := hy
+    use x
+    constructor
+    · simp only [hfx, Option.get_some]
     ·
-      intro h_fam_empty
-      rw [h_fam_empty]
-      simp only [true_or, true_and]
-      unfold partition.mk_if_valid
-      simp only [Finset.not_mem_empty, implies_true, Finset.biUnion_empty, id_eq, true_and, forall_const, imp_self, Option.isSome_some]
-      -- TODO: figure out which tactics were used here
-      simp
+      rw [Finset.mem_filter]
+      constructor
+      · exact hx_in_s
+      · rw [hfx]
+        exact Option.isSome_some
+  -- prove the function is well-defined (implicit argument)
+  .
+    intro x x_in_filter
+    rw [Finset.mem_filter] at x_in_filter
+    exact And.right x_in_filter
+
+lemma partitions_of_empty  {X: Type u} [Inhabited X] [DecidableEq X] :
+  Finset.filterMap
+    (partition.mk_if_valid ∅)
+    { ∅, {∅} }
+    (partition.mk_if_valid_inj_some ∅)
+  = {the_empty_partition X} :=
+by
+  ext part
+  simp only [Finset.mem_filter, Finset.mem_insert, Finset.mem_singleton, or_iff_left_iff_imp, iff_def]
+  constructor
+  · intro fam_part_if_valid
+    ext
+    constructor
+    . intros a_in_fam
+      rw [the_empty_partition]
+      simp only [Finset.not_mem_empty]
+      have : part.family = ∅ :=
+      by
+        unfold partition.mk_if_valid at fam_part_if_valid
+        rw [Finset.mem_filterMap] at fam_part_if_valid
+        rcases fam_part_if_valid with ⟨x, x_partition_if_valid⟩
+        rcases x_partition_if_valid with ⟨x_in_powerset, x_part_if_valid⟩
+        split_ifs at x_part_if_valid with non_empty covers disjoint
+        rw [Option.some_inj] at x_part_if_valid
+        simp only [Finset.mem_insert, Finset.mem_singleton] at x_in_powerset
+        have x_empty_set : x = ∅ := by
+          rcases x_in_powerset with (rfl | x_in_powerset)
+          . exact rfl
+          .
+            exfalso
+            apply absurd non_empty
+            simp only [ne_eq, Finset.forall_mem_not_eq', Decidable.not_not]
+            rw [x_in_powerset]
+            rw [Finset.mem_singleton]
+        obtain ⟨_, _⟩ := x_part_if_valid
+        simp only [x_empty_set]
+      apply absurd a_in_fam
+      rw [this]
+      simp only [Finset.not_mem_empty, not_false_eq_true]
+    unfold the_empty_partition
+    simp only [Finset.not_mem_empty, IsEmpty.forall_iff]
+  .
+    -- TODO: this should be trivialer
+    intro part_empty
+    rcases part_empty with ⟨_, _⟩
+    unfold partition.mk_if_valid
+    rw [Finset.mem_filterMap]
+    use ∅
+    constructor
+    . simp only [Finset.mem_insert, Finset.mem_singleton, true_or]
+    .
+      split_ifs with non_empty covers disjoint
+      rw [Option.some_inj]
+      unfold the_empty_partition
+      rfl
+      .
+        simp only [Finset.not_mem_empty, IsEmpty.forall_iff] at disjoint
+        rw [implies_true, not_true_eq_false] at disjoint
+        exact disjoint
+      . simp only [Finset.biUnion_empty, not_true_eq_false] at covers
+      .
+        simp only [Finset.not_mem_empty, ne_eq, IsEmpty.forall_iff] at non_empty
+        rw [implies_true, not_true_eq_false] at non_empty
+        exact non_empty
+
+lemma card_partitions_of_empty {X: Type u} [Inhabited X] [DecidableEq X] :
+  Fintype.card (partition X ∅) = 1 :=
+by
+  unfold Fintype.card
+  unfold Finset.univ
   unfold Fintype.elems
-  simp
-  rw [empty_double_powerset] at h
-  rw [empty_singleton_powerset]
-  rw [Finset.filterMap]
-  sorry
-
-
+  unfold partition.Fintype
+  simp only [Finset.powerset_empty]
+  rw [singleton_empty_powerset, partitions_of_empty]
+  unfold the_empty_partition
+  rw [Finset.card_singleton]
 
 theorem bell_numbers_count_partitions
   (X : Type u)
